

# Exam 1 Practice Problem Solutions - Spring 2026

1. Let  $\vec{a} = \langle 1, 1, 4 \rangle$  and  $\vec{b} = \langle c, 3, 4 \rangle$ , where  $c$  is an unknown constant.

(a) Find the value of  $c$  so that  $\vec{a}$  and  $\vec{b}$  are orthogonal.

**Solution:** Two vectors  $\vec{a}$  and  $\vec{b}$  are orthogonal if their dot product vanishes, i.e., when  $\vec{a} \cdot \vec{b} = 0$ . If we compute the dot product of the given vectors we obtain

$$(1)(c) + (1)(3) + (4)(4) = 0$$

which implies that  $c + 3 + 16 = 0$ . Therefore,  $c = -19$ .

(b) With the value of  $c$  from part (a), find  $\vec{a} \times \vec{b}$ .

**Solution:** With  $c = -19$ , we have  $\vec{b} = \langle -19, 3, 4 \rangle$ . Now we can compute their cross product:

$$\vec{a} \times \vec{b} = \begin{vmatrix} \mathbf{i} & \mathbf{j} & \mathbf{k} \\ 1 & 1 & 4 \\ -19 & 3 & 4 \end{vmatrix} = \mathbf{i}(4 - 12) - \mathbf{j}(4 - (-76)) + \mathbf{k}(3 - (-19)) = \langle -8, -80, 22 \rangle.$$

So the solution is  $\vec{a} \times \vec{b} = \langle -8, -80, 22 \rangle$ .

2. Find the equation of a line that passes through  $(1, 2, 3)$  and is perpendicular to the plane  $x - y + 3z = 5$ .

**Solution:** The direction vector of the line  $\vec{v}$  is the normal vector of the plane  $\vec{n} = \langle 1, -1, 3 \rangle$ , which we obtain from the coefficients in  $x, y, z$  of the plane  $x - y + 3z = 5$ . Using the point  $(1, 2, 3)$ , the vector equation is:

$$\vec{r}(t) = \langle 1, 2, 3 \rangle + t\langle 1, -1, 3 \rangle$$

Alternative forms:

- Parametric:  $x = 1 + t, y = 2 - t, z = 3 + 3t$ .
- Symmetric:  $x - 1 = 2 - y = \frac{z-3}{3}$ .

3. Find the equation of a plane through the origin,  $(0, 1, 2)$  and  $(3, 0, 1)$ .

**Solution:** Let  $P = (0, 0, 0)$  be the origin, and let  $Q = (0, 1, 2)$ , and  $R = (3, 0, 1)$ . The vectors from  $P$  to  $Q$  and from  $P$  to  $R$  are then given by  $\vec{PQ} = \langle 0, 1, 2 \rangle$  and  $\vec{PR} = \langle 3, 0, 1 \rangle$ . A normal (i.e., perpendicular) vector to  $\vec{PQ}$  and  $\vec{PR}$  can be constructed using the cross product  $\vec{n} = \vec{PQ} \times \vec{PR}$ :

$$\vec{n} = \begin{vmatrix} \mathbf{i} & \mathbf{j} & \mathbf{k} \\ 0 & 1 & 2 \\ 3 & 0 & 1 \end{vmatrix} = \mathbf{i}(1 - 0) - \mathbf{j}(0 - 6) + \mathbf{k}(0 - 3) = \langle 1, 6, -3 \rangle$$

Using the origin as the point  $P$  and the normal vector  $\vec{n}$  we can use the formula for a plane that passes through  $P = (0, 0, 0)$  and is perpendicular to  $\vec{n} = \langle 1, 6, -3 \rangle$  to find the equation of the plane

$$1 \cdot (x - 0) + 6 \cdot (y - 0) - 3 \cdot (z - 0) = 0$$

Thus, the plane we were looking for is  $x + 6y - 3z = 0$ . (The reader can verify that the points  $P$ ,  $Q$ , and  $R$  are in this plane.)

4. Let  $f(x, y)$  be a function satisfying  $f(4, 3) = 5$  and  $\nabla f(4, 3) = \langle 6, 8 \rangle$ .

(a) Find the equation of the tangent plane to  $f$  at  $(4, 3)$ .

**Solution:** The formula for a tangent plane at  $(x_0, y_0, z_0)$  is given by

$$z - z_0 = f_x(x_0, y_0)(x - x_0) + f_y(x_0, y_0)(y - y_0).$$

Since  $\nabla f(x_0, y_0) = \langle f_x(x_0, y_0), f_y(x_0, y_0) \rangle$ , it follows that  $f_x(4, 3) = 6$  and  $f_y(4, 3) = 8$ . Hence, the plane is given by

$$z - 5 = 6(x - 4) + 8(y - 3)$$

which simplifies to the plane  $z = 6x + 8y - 43$ .

(b) Use the linear approximation of  $f(x, y)$  at  $(4, 3)$  to approximate  $f(5, 2)$ .

**Solution:** The linear approximation of  $z = f(x, y)$  at  $(x_0, y_0)$  is given by  $z = L(x, y)$ , the equation of the tangent plane, which we computed to be

$$z = L(x, y) = 5 + 6(x - 4) + 8(y - 3) = 6x + 8y - 43$$

Thus,

$$L(5, 2) = 5 + 6(5 - 4) + 8(2 - 3) = 5 + 6(1) + 8(-1) = 5 + 6 - 8 = 3.$$

So  $f(5, 2) \approx 3$ .

- (c) What is the rate of change of the function at  $(4, 3)$  when moving towards the origin?

**Solution:** The direction vector from  $(4, 3)$  to  $(0, 0)$  is  $\vec{v} = \langle -4, -3 \rangle$ . The magnitude is  $|\vec{v}| = 5$ . Thus, a unit vector in the same direction is given by

$$\vec{u} = \langle -4/5, -3/5 \rangle.$$

Hence the directional derivative in the direction of the unit vector  $\vec{u}$  is given by

$$D_{\vec{u}}f(4, 3) = \nabla f \cdot \vec{u} = \langle 6, 8 \rangle \cdot \langle -4/5, -3/5 \rangle = -24/5 - 24/5 = -48/5 = -9.6.$$

- (d) Which direction maximizes the rate of change of  $f$  at  $(4, 3)$ ?

**Solution:** The rate of change is maximized in the direction of the gradient:  $\nabla f(4, 3) = \langle 6, 8 \rangle$  (or in the direction of the unit vector  $\langle 0.6, 0.8 \rangle$ ).

5. Let  $f(x, y) = \sqrt{x^2 + y^2} \cdot \ln(2x)$ .

- (a) Find the domain of  $f$ .

**Solution:** The square root requires  $x^2 + y^2 \geq 0$  (which holds for all real numbers  $x$  and  $y$ ). The natural log requires  $2x > 0$  and therefore  $x > 0$ . Thus, the domain is  $\{(x, y) \in \mathbb{R}^2 \mid x > 0\}$ .

- (b) Verify by direct computation that  $f_{xy} = f_{yx}$ .

**Solution:** Let  $f = \sqrt{x^2 + y^2} \ln(2x)$ . We compute the first partial derivatives  $f_x$  and  $f_y$  as follows:

$$f_x = \frac{x}{\sqrt{x^2 + y^2}} \ln(2x) + \frac{\sqrt{x^2 + y^2}}{x},$$

$$f_y = \frac{y}{\sqrt{x^2 + y^2}} \ln(2x).$$

Now we compute the mixed second partial derivatives  $f_{yx} = (f_y)_x$  and  $f_{xy} = (f_x)_y$  as follows

$$f_{yx} = \frac{\partial}{\partial x}(f_y) = y \ln(2x) \cdot \frac{-x}{(x^2 + y^2)^{3/2}} + \frac{y}{\sqrt{x^2 + y^2}} \cdot \frac{1}{x} = \frac{y}{x\sqrt{x^2 + y^2}} - \frac{xy \ln(2x)}{(x^2 + y^2)^{3/2}}$$

$$f_{xy} = \frac{\partial}{\partial y}(f_x) = x \ln(2x) \cdot \frac{-y}{(x^2 + y^2)^{3/2}} + \frac{1}{x} \cdot \frac{y}{\sqrt{x^2 + y^2}} = \frac{y}{x\sqrt{x^2 + y^2}} - \frac{xy \ln(2x)}{(x^2 + y^2)^{3/2}}.$$

Thus, we have verified that  $f_{xy} = f_{yx}$ .

6. Let  $f(x, y) = (x^2 - y^2)e^y$  and let  $g(t) = \cos(t)$  and  $h(t) = \sin(t)$ . Use the chain rule to compute the derivative with respect to  $t$  of the function  $f(g(t), h(t))$ .

**Solution:** The multivariable one-parameter chain rule says that

$$\frac{df}{dt} = \frac{\partial f}{\partial x} \frac{dx}{dt} + \frac{\partial f}{\partial y} \frac{dy}{dt}.$$

First we compute some partial derivatives:

$$f_x = 2xe^y, f_y = -2ye^y + (x^2 - y^2)e^y = (x^2 - y^2 - 2y)e^y,$$

and one-variable derivatives:

$$\frac{dx}{dt} = -\sin(t), \frac{dy}{dt} = \cos(t).$$

Thus,

$$\frac{df}{dt} = (2 \cos t e^{\sin t})(-\sin t) + (\cos^2 t - \sin^2 t - 2 \sin t)e^{\sin t}(\cos t).$$

7. Let  $f$  be a continuous function of two variables which is twice differentiable with the following table of values.

|            | $f(x, y)$ | $f_x(x, y)$ | $f_y(x, y)$ | $f_{xx}(x, y)$ | $f_{xy}(x, y)$ | $f_{yy}(x, y)$ |
|------------|-----------|-------------|-------------|----------------|----------------|----------------|
| $(-1, 2)$  | 11        | 0           | 0           | 1              | 5              | 3              |
| $(1, 4)$   | -5        | 1           | 0           | 2              | 0              | 4              |
| $(-2, -1)$ | 6         | 0           | 0           | -3             | 0              | -1             |
| $(-4, -1)$ | 0         | 2           | 2           | 1              | 0              | 1              |
| $(1, -3)$  | 2         | 3           | 0           | -2             | 5              | 2              |

- (a) Which points are critical points?

**Solution:** Critical points occur where  $f_x = 0$  and  $f_y = 0$ . Looking at the table, these are A:  $(-1, 2)$  and C:  $(-2, -1)$ .

- (b) Classify each critical point.

**Solution:** Use Second Derivative Test, using the auxiliary value  $D = f_{xx}f_{yy} - (f_{xy})^2$ .

- For  $(-1, 2)$  :  $D = (1)(3) - (5)^2 = 3 - 25 = -22$ . Since  $D = D(-1, 2) < 0$ , it is a **Saddle Point**.
- For  $(-2, -1)$  :  $D(-2, -1) = (-3)(-1) - (0)^2 = 3$ . Since  $D = D(-2, -1) > 0$  and  $f_{xx} = -3 < 0$ , it is a **Local Maximum**.

8. Use the method of *Lagrange Multipliers* to find the maximum and the minimum of  $f(x, y) = x^2 + y$  over the ellipse  $x^2 + 2y^2 = 8$ .

**Solution:** The method of Lagrange Multipliers says that the max and min will happen at those points such that  $\nabla f = \lambda \nabla g$ . We first compute the gradient vectors:

$$\nabla f = \langle 2x, 1 \rangle, \text{ and } \nabla g = \langle 2x, 4y \rangle.$$

By setting  $\nabla f = \lambda \nabla g$  we obtain  $\langle 2x, 1 \rangle = \lambda \langle 2x, 4y \rangle$ . Thus, we obtain two equations:

$$2x = 2x\lambda \text{ and } 1 = 4y\lambda.$$

Since  $2x = 2x\lambda$  implies  $2x(1 - \lambda) = 0$  we have two cases to consider

- Case 1:  $x = 0$ .
- Case 2:  $\lambda = 1$ .

If  $x = 0$ , then  $0^2 + 2y^2 = 8$  implies  $y^2 = 4$  which in turn implies that  $y = \pm 2$ . We obtain two points:  $(0, 2), (0, -2)$ .

If  $\lambda = 1$ , then  $1 = 4y \cdot 1$  implies  $y = 1/4$ . Moreover the point is on the ellipse so  $x^2 + 2(1/4)^2 = 8$  which implies  $x^2 + 1/8 = 8$  and so  $x^2 = 63/8$ . Thus,  $x = \pm\sqrt{7.875}$ . We obtain another two points  $(\pm\sqrt{63/8}, 1/4)$ .

Finally we evaluate  $f$  at the points we found:  $f(0, 2) = 2$ ,  $f(0, -2) = -2$ ,  $f(\pm\sqrt{63/8}, 1/4) = 7.875 + 0.25 = 8.125$ .

Hence, the **Max value** is 8.125 at  $(\pm\sqrt{63/8}, 1/4)$  and the **Min value** is -2 at  $(0, -2)$ .